wavl_noninter.mli
@@ -1,9 +1,4 @@
 
-type comparison =
-| Eq
-| Lt
-| Gt
-
 type compareSpecT =
 | CompEqT
 | CompLtT
@@ -14,11 +9,9 @@ type 'a sig0 = 'a
 
 
 
-type 'a ordered = { compare : ('a -> 'a -> comparison); compare_spec : ('a -> 'a -> compareSpecT) }
-
 type a (* AXIOM TO BE REALIZED *)
 
-val ordA : a ordered
+val compare_spec : a -> a -> compareSpecT
 
 type wavltree =
 | Node of bool * a * wavltree * wavltree
