ordered.v
@@ -25,10 +25,105 @@ WITH THE SOFTWARE OR THE USE OR OTHER DEALINGS IN THE SOFTWARE.
 
 Require Export Coq.Classes.RelationClasses.
 
-Class Ordered(A : Set) := 
-  {
-    lt : A -> A -> Prop;
-    lt_strict :> StrictOrder lt;
-    compare : A -> A -> comparison;
-    compare_spec : forall x y, CompareSpecT (eq x y) (lt x y) (lt y x) (compare x y)
+Set Default Goal Selector "all".
+
+Class Ordered(A : Set) :=
+  { lt : A -> A -> Prop;
+    lt_strict :> StrictOrder lt
   }.
+
+Class OrderedKeyed (A K : Set) :=
+  { keyof : A -> K;
+    OA :> Ordered A
+  }.
+
+Class KeyOrdered (A K : Set) :=
+  { getkey : A -> K;
+    OK :> Ordered K
+  }.
+
+Definition KOlt{A K : Set}`{KeyOrdered A K}(a b : A) : Prop := lt (getkey a) (getkey b).
+
+Instance KOisO A K `{KeyOrdered A K} : Ordered A.
+Proof.
+  destruct (_:KeyOrdered A K) as [gk [ltk [SOI SOT]]]. unshelve eexists.
+  - intros a b. exact (ltk (gk a) (gk b)).
+  - split.
+    + unfold Irreflexive, Reflexive, complement in *. intro. apply SOI.
+    + unfold Transitive in *. intros x y z. apply SOT.
+Defined.
+
+Instance KOisOK A K `{KeyOrdered A K} : OrderedKeyed A K :=
+  { keyof := getkey }.
+
+Class ComparableKeyed (A K : Set) :=
+  { OKOK :> OrderedKeyed A K;
+    compare : K -> K -> comparison;
+    compare_spec x y: CompareSpecT (eq x y)
+                                   (forall (a b : A), x = keyof a -> y = keyof b -> lt a b)
+                                   (forall (a b : A), x = keyof a -> y = keyof b -> lt b a)
+                                   (compare x y);
+    lt_same_keys w x y z: lt w y -> keyof x = keyof w -> keyof z = keyof y -> lt x z
+  }.
+
+Require Coq.Init.Nat.
+Require Coq.Arith.PeanoNat.
+
+Module Test.
+
+  Import Nat.
+  Import PeanoNat.
+  
+  Open Scope nat_scope.
+
+  Context {A : Set}.
+  Context {Ord : Ordered A}.
+
+  Record OK : Set := { val : A; key : nat }.
+
+  Definition OKlt (a b : OK) : Prop := a.(key) < b.(key).
+
+  Lemma le_Sn_n : forall n, S n <= n -> False.
+  Proof.
+    induction n as [|? IHn]. intro H.
+    - inversion H.
+    - apply IHn. apply le_S_n. assumption.
+  Qed.
+
+  Lemma OKlt_strict : StrictOrder OKlt.
+  Proof.
+    eexists. red.
+    - red. red. intros [v k]. cbv. apply le_Sn_n.
+    - intros [? ?] [? ykey] [? ?]. unfold OKlt, key. transitivity ykey. assumption.
+  Qed.
+
+  Instance OKOrd : Ordered OK := { lt := OKlt; lt_strict := OKlt_strict }.
+
+  Lemma OKOrd_compare_spec (x y:nat) :
+    CompareSpecT (eq x y)
+                 (forall (a b : OK), x = a.(key) -> y = b.(key) -> OKlt a b)
+                 (forall (a b : OK), x = a.(key) -> y = b.(key) -> OKlt b a)
+                 (Nat.compare x y).
+  Proof.
+    destruct (CompareSpec2Type (Nat.compare_spec x y)). constructor.
+    - assumption.
+    - intros ? ? -> -> . assumption.
+    - intros ? ? -> -> . assumption.
+  Qed.
+
+  Lemma OKOrd_lt_same_keys w x y z :
+    OKlt w y -> x.(key) = w.(key) -> z.(key) = y.(key) -> OKlt x z.
+  Proof.
+    unfold OKlt. intros H -> -> . assumption.
+  Qed.
+
+  Instance OKnat : OrderedKeyed OK nat := { keyof := key }.
+ 
+  Instance CKnat : ComparableKeyed OK nat :=
+    { compare := Nat.compare;
+      compare_spec := OKOrd_compare_spec;
+      lt_same_keys := OKOrd_lt_same_keys
+    }.
+
+End Test.
+
