hypiter.v
@@ -23,181 +23,23 @@ WITH THE SOFTWARE OR THE USE OR OTHER DEALINGS IN THE SOFTWARE.
 
  ***********************************************************************)
 
-(*Iteration over Hypotheses
+(*Iteration over Hypotheses *)
 
-In order to simplify iteration over hypotheses in a goal, we first "harvest"
-together the hyps into a single term that can be easily pulled apart one hyp
-at a time.  There is a very simple way to do this using the fact that the
-constructor tactic can can construct a function of any number of arguments of
-any type that returns some easily constructed type, such as True.  We then use
-the tactic-in-term construct ltac:(...) to create the desired goal type by
-reverting or generalizing the hyptheses we want to be part of it.  The
-resulting constr will be a function application, where the hyps are the args -
-and so can be popped off at the right.  *)
+(*fast non-kludgy versions of iteration:*)
+Ltac allhyps_bu tac := (*tac runs in bottom-up hyp order*)
+  let rec f icont tcont :=
+      idtac;
+      lazymatch goal with
+      | H : _ |- _ => revert H; f ltac:(intro H; icont) ltac:(tcont; tac H)
+      | _ => icont; tcont
+      end
+  in f ltac:(idtac) ltac:(idtac).
 
-Ltac harvest_hyps harvester :=
-  constr:(ltac:(harvester; constructor) : True).
-
-Tactic Notation "harvest" tactic3(harvester) "=>" tactic3(tac) :=
-  (* Typical harvesters are "generalize hs" and "revert_clearbody_all" *)
-  let hs := harvest_hyps harvester in
-  tac hs.
-
-Ltac last_hyp :=
-  lazymatch goal with H : _ |- _ => H end.
-
-Ltac revert_clearbody H := try clearbody H; revert H.
-
-Ltac revert_clearbody_all :=
-  repeat revert_clearbody last_hyp.
-
-Ltac all_hyps := harvest_hyps revert_clearbody_all.
-
-(*All hyps in the usual bottom-up order:*)
-Tactic Notation "hyps" "=>" tactic3(tac) :=
-  harvest revert_clearbody_all => tac.
-
-(*Just the specified hyps*)
-Tactic Notation "hyps" ne_hyp_list(hs) "=>" tactic3(tac) :=
-  harvest generalize hs => tac.
-
-(*next_hyp is the basic iteration-building component for iterating
-over hypotheses*)
-Ltac next_hyp hs step last := 
-  lazymatch hs with 
-  | (?hs' ?H) => step H hs'
-  | _ => last
-  end.
-
-(*Normal forward loop (bottom-up hypotheses)
-For example, to loop over all hyps:
-  hyps => loop tac.
-where tac is a function of a single hyp.
-*)
-Ltac loop tac hs :=
-  idtac;
-  let rec step H hs := tac H; next_hyp hs step idtac in
-  next_hyp hs step idtac.
-
-Ltac next_hyp2 hs step acc :=
-  lazymatch hs with
-  | (?hs' ?H) => step H acc hs'
-  | _ => acc
-  end.
-
-Ltac ufold tac acc hs :=
-  let rec step H a hs := let b:=tac H a in next_hyp2 hs step b in
-  next_hyp2 hs step acc.
-
-Ltac dfold tac acc hs :=
-  let rec step H a hs := let b:=next_hyp2 hs step a in tac H b in
-  next_hyp2 hs step acc.
-
-(*Forward iteration that stops instead of failing when tac fails at
-level 0 (fail higher to undo the iteration) *)
-Ltac tryloop tac hs :=
-  idtac;
-  let rec step H hs := 
-      tryif tac H then next_hyp hs step idtac else idtac in
-  next_hyp hs step idtac.
-
-(*Forward iteration with a separate cond test - iteration of tac
-continues while cond is true. *)
-Ltac while cond tac hs :=
-  idtac;
-  let rec step H hs := 
-      tryif cond H then tac H; next_hyp hs step idtac else idtac in
-  next_hyp hs step idtac.
-
-(*Similar iterator variants (try, while) are possible with the
-following as well:*)
-
-(*Normal reverse loop (top-down hypotheses) *)
-Ltac rloop tac hs :=
-  idtac;
-  let rec step H hs := next_hyp hs step idtac; tac H in
-  next_hyp hs step idtac.
-
-(*Backtrack-capable choice*)
-Ltac plusses tac hs :=
-  idtac;
-  let rec step H hs := tac H + next_hyp hs step fail in
-  next_hyp hs step fail.
-
-(*Non-backtrack-cabable choice via first*)
-Ltac firsts tac hs :=
-  idtac;
-  let rec step H hs := first[tac H | next_hyp hs step fail] in
-  next_hyp hs step fail.
-
-(*Non-backtrack-capable choice via ||*)
-Ltac bars tac hs :=
-  idtac;
-  let rec step H hs := tac H || next_hyp hs step fail in
-  next_hyp hs step fail.
-
-(*Other interesting hyp harvester functions:*)
-
-Ltac clear_through H :=
-  let H':= last_hyp in
-  clear H';
-   first[ constr_eq H' H 
-        | clear_through H].
-
-Ltac revert_clearbody_below H :=
-  let H':=last_hyp in
-  first [ constr_eq H' H
-        | try clearbody H';
-          revert H'; 
-          revert_clearbody_below H].
-
-(*Modifiers of harvested hypotheses:*)
-
-(*negation*)
-Ltac neg tac hs :=
-  idtac;
-  let gen_if_absent H := 
-      match hs with context[H] => idtac | _ => generalize H end in
-  harvest (hyps => loop gen_if_absent) => tac.
-
-(*With negation, we can do hyps -, which excludes specific hyps:*)
-Tactic Notation "hyps" "-" hyp_list(hs) "=>" tactic3(tac) :=
-  harvest generalize hs => neg tac.
-
-(*inclusion based on predicate (filt)*)
-Ltac filter filt tac hs :=
-  let g H := idtac;tryif filt H then generalize H else idtac in
-  harvest loop g hs => tac.
-
-(*inclusion based on type*)
-Ltac filter_type type :=
-  let filt H := let tH:=type of H in constr_eq tH type in
-  filter filt.
-
-Ltac gen H := generalize H.
-
-(*inclusion based on position above hyp H*)
-Ltac above H tac hs :=
-  idtac;
-  let gen := clear_through H; loop gen hs in
-  harvest gen => tac.
-
-(*inclusion based on position below hyp H*)
-Ltac below H tac hs :=
-  harvest revert_clearbody_below H => tac.
-
-(*adding H to front of iteration*)
-Ltac firstly H tac hs :=
-  idtac;
-  let gen := generalize H; loop gen hs in
-  harvest gen => tac.
-
-(*adding H to back of iteration*)
-Ltac lastly H tac hs :=
-  idtac;
-  let g := loop gen hs; generalize H in
-  harvest g => tac.
-
-(*reversing the order*)
-Ltac reverse tac hs :=
-  harvest rloop gen hs => tac.
+Ltac allhyps_td tac := (*tac runs in top-down hyp order*)
+  let rec f icont tcont :=
+      idtac;
+      lazymatch goal with
+      | H : _ |- _ => revert H; f ltac:(intro H; icont) ltac:(tac H; tcont)
+      | _ => icont; tcont
+      end
+  in f ltac:(idtac) ltac:(idtac).
